\section{Law}
%%%%%%%%%%%%%%%%%%%%%%%%%%%%%%%%
\subsection{Exponents}
\begin{enumerate}
	\item
	\[a^m \; \times \; a^n \; = a^{m+n} \qquad (m, \; n \in \mathbb{N})\] \[a^m \; \times \; a^n \; = a^{m+n} \qquad (m, \; n \in \mathbb{Z}; \; a \neq 0, \; if \quad m \quad or \quad n \; < \; 0)\]
	\item
	\[\frac{a^m}{a^n}=a^{m-n} \qquad (m, \; n \in \mathbb{Z}; \; a \in \mathbb{R}; \; a \neq 0)\]
	\item
	\[(ab)^m \; = \; a^m \; b^m \qquad (m \in \mathbb{Z})\]
	\item
	\[(a^m)^n \; = \; a^{mn} \qquad (m, \; n \in \mathbb{Z})\]
\end{enumerate}
%%%%%%%%%%%%%%%%%%%%%%%%%%%%%%%%
\subsection{Rational Exponents}
\begin{enumerate}
	\item
	\[a^r \; \times \; a^t \; = \; a^{r+t} \qquad (a \; > \; 0; \quad r, \; t \in \mathbb{Q})\]
	\item
	\[\frac{a^r}{a^t}=a^{r-t} \qquad (a \; > \; 0; \quad r, \;t \in \mathbb{Q})\]
	\item
	\[(a^t)^r \; = \; a^{tr} \qquad (a \; > \; 0, \quad t, \; r \in \mathbb{Q})\]
	\item
	\[(ab)^t \; = \; a^t \; b^t \; ; \quad \left(\frac{a}{b}\right)^t \; = \; \frac{a^t}{b^t} \; ; \qquad (a, \; b \; > \; 0, \quad t \in \mathbb{Q})\]
	\[\hspace{1cm} and :\]
	\[\hspace{3cm} a^t \; b^t \; = \; (ab)^t \qquad and \qquad \frac{a^t}{b^t} \; = \; \left(\frac{a}{b}\right)^t\]
\end{enumerate}
%%%%%%%%%%%%%%%%%%%%%%%%%%%%%%%%
\subsection{Distributive law}
\[a(b \; + \; c) \; = \; ab \; + \; ac\]
\begin{align*}
	(a \; + \; b)(c \; + \; d) \; &= \; (a \; + \; b)c \; + \; (a \; + \; b)d \\
	&=ac \; + \;bc \; + \; ad \; + \; bd
\end{align*}
\[A^2 \; - \; B^2 \; = \; (A \; - \; B)(A \; + \; B)\]
%%%%%%%%%%%%%%%%%%%%%%%%%%%%%%%%
\subsection{Commutative law}
\[ab \; = \; ba\]
%%%%%%%%%%%%%%%%%%%%%%%%%%%%%%%%
%%%%%%%%%%%%%%%%%%%%%%%%%%%%%%%%%%%%%%%%%%%%%%%%%%%%%%%%%%%%%%%%%%%%%
