\documentclass[12pt]{article}
\usepackage{amsmath, amssymb}
\usepackage{geometry}
\usepackage{booktabs}
\usepackage{parskip}
\usepackage{titlesec}
\usepackage{fancyhdr}
\geometry{margin=0.85in}
\pagestyle{fancy}
\fancyhf{}
\rhead{\thepage}
\lhead{Calculus Reference}

\titleformat{\section}{\large\bfseries}{}{0pt}{}
\titleformat{\subsection}{\normalsize\bfseries}{}{0pt}{}

\begin{document}

\section*{Derivative Formulas}

\subsection*{Basic Rules}
\begin{tabular}{@{}ll@{}}
\toprule
$\displaystyle \frac{d}{dx}(c)$ & $= 0$ \\
$\displaystyle \frac{d}{dx}(x)$ & $= 1$ \\
$\displaystyle \frac{d}{dx}[cf(x)]$ & $= c \cdot f'(x)$ \\
$\displaystyle \frac{d}{dx}[f \pm g]$ & $= f' \pm g'$ \\
$\displaystyle \frac{d}{dx}[fg]$ & $= f'g + fg'$ \\
$\displaystyle \frac{d}{dx}\left[\frac{f}{g}\right]$ & $= \frac{f'g - fg'}{g^2}$ \\
\bottomrule
\end{tabular}

\vspace{1em}
\subsection*{Power and Root}
\begin{tabular}{@{}ll@{}}
\toprule
$\displaystyle \frac{d}{dx}(x^n)$ & $= nx^{n-1}$ \\
$\displaystyle \frac{d}{dx}(\sqrt{x})$ & $= \frac{1}{2\sqrt{x}}$ \\
$\displaystyle \frac{d}{dx}(x^{1/n})$ & $= \frac{1}{n}x^{\frac{1}{n}-1}$ \\
\bottomrule
\end{tabular}

\vspace{1em}
\subsection*{Exponential and Logarithmic}
\begin{tabular}{@{}ll@{}}
\toprule
$\displaystyle \frac{d}{dx}(e^x)$ & $= e^x$ \\
$\displaystyle \frac{d}{dx}(a^x)$ & $= a^x \ln a$ \\
$\displaystyle \frac{d}{dx}(\ln x)$ & $= \frac{1}{x}$ \\
$\displaystyle \frac{d}{dx}(\log_a x)$ & $= \frac{1}{x \ln a}$ \\
\bottomrule
\end{tabular}

\vspace{1em}
\subsection*{Trigonometric}
\begin{tabular}{@{}ll@{}}
\toprule
$\displaystyle \frac{d}{dx}(\sin x)$ & $= \cos x$ \\
$\displaystyle \frac{d}{dx}(\cos x)$ & $= -\sin x$ \\
$\displaystyle \frac{d}{dx}(\tan x)$ & $= \sec^2 x$ \\
$\displaystyle \frac{d}{dx}(\cot x)$ & $= -\csc^2 x$ \\
$\displaystyle \frac{d}{dx}(\sec x)$ & $= \sec x \tan x$ \\
$\displaystyle \frac{d}{dx}(\csc x)$ & $= -\csc x \cot x$ \\
\bottomrule
\end{tabular}

\vspace{1em}
\subsection*{Inverse Trigonometric}
\begin{tabular}{@{}ll@{}}
\toprule
$\displaystyle \frac{d}{dx}(\sin^{-1}x)$ & $= \frac{1}{\sqrt{1 - x^2}}$ \\
$\displaystyle \frac{d}{dx}(\cos^{-1}x)$ & $= -\frac{1}{\sqrt{1 - x^2}}$ \\
$\displaystyle \frac{d}{dx}(\tan^{-1}x)$ & $= \frac{1}{1 + x^2}$ \\
$\displaystyle \frac{d}{dx}(\cot^{-1}x)$ & $= -\frac{1}{1 + x^2}$ \\
$\displaystyle \frac{d}{dx}(\sec^{-1}x)$ & $= \frac{1}{|x|\sqrt{x^2 - 1}}$ \\
$\displaystyle \frac{d}{dx}(\csc^{-1}x)$ & $= -\frac{1}{|x|\sqrt{x^2 - 1}}$ \\
\bottomrule
\end{tabular}

\newpage

\section*{Integral Formulas}

\subsection*{Basic Rules}
\begin{tabular}{@{}ll@{}}
\toprule
$\displaystyle \int c\,dx$ & $= cx + C$ \\
$\displaystyle \int x^n\,dx$ & $= \frac{x^{n+1}}{n+1} + C$ \quad ($n \ne -1$) \\
$\displaystyle \int \frac{1}{x}\,dx$ & $= \ln|x| + C$ \\
\bottomrule
\end{tabular}

\vspace{1em}
\subsection*{Exponential and Logarithmic}
\begin{tabular}{@{}ll@{}}
\toprule
$\displaystyle \int e^x\,dx$ & $= e^x + C$ \\
$\displaystyle \int a^x\,dx$ & $= \frac{a^x}{\ln a} + C$ \\
$\displaystyle \int \ln x\,dx$ & $= x\ln x - x + C$ \\
\bottomrule
\end{tabular}

\vspace{1em}
\subsection*{Trigonometric}
\begin{tabular}{@{}ll@{}}
\toprule
$\displaystyle \int \sin x\,dx$ & $= -\cos x + C$ \\
$\displaystyle \int \cos x\,dx$ & $= \sin x + C$ \\
$\displaystyle \int \tan x\,dx$ & $= -\ln|\cos x| + C$ \\
$\displaystyle \int \cot x\,dx$ & $= \ln|\sin x| + C$ \\
$\displaystyle \int \sec x\,dx$ & $= \ln|\sec x + \tan x| + C$ \\
$\displaystyle \int \csc x\,dx$ & $= -\ln|\csc x + \cot x| + C$ \\
\bottomrule
\end{tabular}

\vspace{1em}
\subsection*{Inverse Trigonometric}
\begin{tabular}{@{}ll@{}}
\toprule
$\displaystyle \int \frac{1}{\sqrt{1 - x^2}}\,dx$ & $= \sin^{-1}x + C$ \\
$\displaystyle \int \frac{1}{1 + x^2}\,dx$ & $= \tan^{-1}x + C$ \\
$\displaystyle \int \frac{1}{x\sqrt{x^2 - 1}}\,dx$ & $= \sec^{-1}|x| + C$ \\
\bottomrule
\end{tabular}

\vspace{1em}
\subsection*{(Optional) Hyperbolic}
\begin{tabular}{@{}ll@{}}
\toprule
$\displaystyle \int \sinh x\,dx$ & $= \cosh x + C$ \\
$\displaystyle \int \cosh x\,dx$ & $= \sinh x + C$ \\
\bottomrule
\end{tabular}

\end{document}
