\documentclass[fleqn]{article}
\usepackage{amsmath,amssymb}
\usepackage[margin=1in]{geometry}
\usepackage{multicol}
\setlength{\mathindent}{0pt} % flush left math

\pagestyle{empty}

\begin{document}

\begin{center}
  {\LARGE \textbf{Laplace and Inverse Laplace Formulas}}\\[6pt]
  \rule{\linewidth}{0.5pt}
\end{center}

\begin{multicols}{2}
\small

% Laplace Transform
\section*{$\mathcal{L}\{f(t)\} = F(s)$}

\[
\mathcal{L}\{1\} = \frac{1}{s}, \quad s>0
\]

\[
\mathcal{L}\{t^n\} = \frac{n!}{s^{n+1}}, \quad n=0,1,2,\dots
\]

\[
\mathcal{L}\{e^{at}\} = \frac{1}{s - a}, \quad s > a
\]

\[
\mathcal{L}\{\sin(\omega t)\} = \frac{\omega}{s^2 + \omega^2}
\]

\[
\mathcal{L}\{\cos(\omega t)\} = \frac{s}{s^2 + \omega^2}
\]

\[
\mathcal{L}\{\sinh(\omega t)\} = \frac{\omega}{s^2 - \omega^2}, \quad s > |\omega|
\]

\[
\mathcal{L}\{\cosh(\omega t)\} = \frac{s}{s^2 - \omega^2}, \quad s > |\omega|
\]

\[
\mathcal{L}\{t^n e^{at}\} = \frac{n!}{(s - a)^{n+1}}, \quad s > a
\]

\[
\mathcal{L}\{u(t - a)\} = \frac{e^{-a s}}{s}, \quad a \ge 0
\]

\[
\mathcal{L}\{\delta(t - a)\} = e^{-a s}
\]

\vspace{6pt}

% Inverse Laplace Transform
\section*{$\mathcal{L}^{-1}\{F(s)\} = f(t)$}

\[
\mathcal{L}^{-1}\left\{\frac{1}{s}\right\} = 1
\]

\[
\mathcal{L}^{-1}\left\{\frac{n!}{s^{n+1}}\right\} = t^n, \quad n=0,1,2,\dots
\]

\[
\mathcal{L}^{-1}\left\{\frac{1}{s - a}\right\} = e^{at}
\]

\[
\mathcal{L}^{-1}\left\{\frac{\omega}{s^2 + \omega^2}\right\} = \sin(\omega t)
\]

\[
\mathcal{L}^{-1}\left\{\frac{s}{s^2 + \omega^2}\right\} = \cos(\omega t)
\]

\[
\mathcal{L}^{-1}\left\{\frac{\omega}{s^2 - \omega^2}\right\} = \sinh(\omega t)
\]

\[
\mathcal{L}^{-1}\left\{\frac{s}{s^2 - \omega^2}\right\} = \cosh(\omega t)
\]

\[
\mathcal{L}^{-1}\left\{\frac{n!}{(s - a)^{n+1}}\right\} = t^n e^{at}, \quad n=0,1,2,\dots
\]

\[
\mathcal{L}^{-1}\left\{ \frac{e^{-a s}}{s} \right\} = u(t - a)
\]

\[
\mathcal{L}^{-1}\left\{e^{-a s}\right\} = \delta(t - a)
\]

\end{multicols}

\end{document}
